\documentclass[a4paper]{article}

\usepackage{fontspec}
\usepackage{mathpazo}
\setmainfont
     [ BoldFont       = texgyrepagella-bold.otf ,
       ItalicFont     = texgyrepagella-italic.otf ,
       BoldItalicFont = texgyrepagella-bolditalic.otf ]
     {texgyrepagella-regular.otf}
\setmainfont{Gill Sans MT}

\usepackage[english]{babel}
\usepackage[utf8]{inputenc}
\usepackage{amsmath}
\usepackage{graphicx}
\usepackage[colorinlistoftodos]{todonotes}
\usepackage{physics}

\title{Math Dump}

\author{David McPherson}

\date{\today}

\begin{document}

\section{Poster Math}
  \subsection{Abate}

  \begin{align*}
  \dot{x} = f(x) + g(x) u + b
  \end{align*}

  \begin{align*}
  \dot{x}_1 &= x_2
  \\
  \dot{x}_2 &= k_t u^2 + g + b
  \end{align*}

  \begin{align*}
  V_{k-1} & = \mathbf{1_A}(x) \mathrm{E}_{z \sim T} (V(z))
  \\ & = \mathbf{1_A}(x) \mathrm{E}_{b\sim N} (V( x + (f(x) + g(x) u + b) \Delta t) )
  \\ & = \mathbf{1_A}(x) \int_{-\infty}^{\infty} V( x + (f(x) + g(x) u + b) \Delta t) \frac{1}{\sigma \sqrt{2 \pi}} e^{-\frac{(x-\mu)^2}{2 \sigma^2}} db
  \end{align*}

  \subsection{Differential Form}

  \begin{align*}
  V_{k-1}(x) & = \mathbf{1_A}(x) \mathrm{E}_{z \sim T} (V_k(z))
  \\ & = \mathbf{1_A}(x) \mathrm{E}_{b\sim N} (V_k( x + (f(x) + g(x) u + b) \Delta t) )
  \\ & = \mathbf{1_A}(x) \mathrm{E}_{b\sim N} (V_k( x ) + \nabla V_k^T (f(x) + g(x) u + b) \Delta t )
  \\ & = \mathbf{1_A}(x) V_k(x) + \mathrm{E}_{b\sim N} ( \nabla V_k^T (f(x) + g(x) u + b) \Delta t )
  \\ & = \mathbf{1_A}(x) V_k(x) + \nabla V_k^T \mathrm{E}_{b\sim N} ( f(x) + g(x) u + b ) \Delta t
  \\ \rightarrow
  \\ \frac{V_{k-1} - V_k(x)}{\Delta t} &= \nabla V_k^T \mathrm{E}_{b\sim N} ( f(x) + g(x) u + b )
  \end{align*}

  \begin{align*}
  \\ \Delta t \rightarrow 0
  \\ -\frac{\delta V}{\delta t} &= \nabla V_k^T \mathrm{E}_{b\sim N} ( f(x) + g(x) u + b )
  \\ -\frac{\delta V}{\delta t} &= \nabla V_k^T ( f(x) + g(x) u + \mu )
  \end{align*}

  \subsection{Mitchell Magic}

  \begin{align*}
  dx &= F(x,u) dt + \sigma(x) dB
  \end{align*}
  \begin{align*}
  -\frac{\delta V}{\delta t} = \nabla V_k^T \mathrm{E}_{b\sim N} ( f(x) + g(x) u + b ) + 0.5 \texttt{trace} [\sigma(x) \sigma(x)^T \nabla^2_x V_k]
  \end{align*}
  \begin{align*}
  dx &= (f(x) + g(x) u + \mu(x) ) dt + \sigma(x) dB
  \end{align*}

\section{Writeup Temp}

\begin{align}
V_{k-1}(x) & = \mathbf{1_A}(x) \mathrm{E}_{z \sim P(x_k = z | x_{k-1}=x)} (V_k(z))
\\ & = \mathbf{1_A}(x) \mathrm{E}_{b_k\sim N} (V_k( x + (f(x) + g(x) u_k + \mu(x)) \Delta t + \sigma(x) \sqrt{\Delta t} b_k )
\\ & = \mathbf{1_A}(x) \mathrm{E}_{b\sim N} (V_k( x ) + \nabla V_k^T ((f(x) + g(x) u_k + \mu(x)) \Delta t + \sigma(x) \sqrt{\Delta t} b_k) )
\\ & = \mathbf{1_A}(x) V_k(x) + \mathrm{E}_{b\sim N} ( \nabla V_k^T ( (f(x) + g(x) u_k + \mu(x)) \Delta t + \sigma(x) \sqrt{\Delta t} b_k)  )
\\ & = \mathbf{1_A}(x) V_k(x) + \nabla V_k^T \mathrm{E}_{b\sim N}   ( (f(x) + g(x) u_k + \mu(x)) \Delta t + \sigma(x) \sqrt{\Delta t} b_k)
\\ & = \mathbf{1_A}(x) V_k(x) + \nabla V_k^T \mathrm{E}_{b\sim N}   ( (f(x) + g(x) u_k + \mu(x)) \Delta t + \sigma(x) \sqrt{\Delta t} b_k)
\\ \rightarrow
\\ \frac{V_{k-1} - V_k(x)}{\Delta t} &= \nabla V_k^T \mathrm{E}_{b\sim N} ( f(x) + g(x) u + b )
\end{align}

\end{document}
